Split apart LN/DB roundtrip and start to verify actual bijection

Tealeaves/Backends/Adapters/LNtoDB.v
@@ -26,8 +26,6 @@ From Tealeaves Require Import
   Backends.Adapters.Key
   Functors.Option.
 
-
-
 Import LN.Notations.
 
 Import DecoratedTraversableMonad.UsefulInstances.
@@ -45,13 +43,6 @@ Definition toDB_loc (k: key) '(depth, l) : option nat :=
   | Bd n => Some n
   | Fr x => map (fun ix => ix + depth) (key_lookup_atom k x)
   end.
-
-Definition toLN_loc (k: key) '(depth, ix) : option LN :=
-  if bound ix depth == true
-  then
-    Some (Bd ix)
-  else
-    map (F := option) Fr (key_lookup_index k (ix - depth)).
 
 Fixpoint toLNkey_list (l: list LN): key :=
   match l with
@@ -100,6 +91,7 @@ Proof.
   apply key_bijection.
   apply toLNkey_unique.
 Qed.
+
 (*|
 ============================
 Global operations
@@ -109,10 +101,6 @@ Definition toDB_from_key
   `{Mapdt_inst: Mapdt nat T} (k: key): T LN -> option (T nat) :=
   mapdt (G := option) (toDB_loc k).
 
-Definition toLN_from_key
-  `{Mapdt_inst: Mapdt nat T} (k: key): T nat -> option (T LN) :=
-  mapdt (G := option) (toLN_loc k).
-
 Definition toLNkey
   `{Traverse_inst: Traverse T} (t: T LN): key :=
   toLNkey_list (tolist t).
@@ -121,250 +109,3 @@ Definition toDB
   `{Traverse_inst: Traverse T}
   `{Mapdt_inst: Mapdt nat T} (t: T LN): option (T nat) :=
   toDB_from_key (toLNkey t) t.
-
-Section translate.
-
-  Context
-    `{Return_T: Return T}
-    `{Binddt_TT: Binddt nat T T}
-    `{Binddt_TU: Binddt nat T U}
-    `{Monad_inst: ! DecoratedTraversableMonad nat T}
-    `{Module_inst: ! DecoratedTraversableRightPreModule nat T U
-                        (unit := Monoid_unit_zero)
-                        (op := Monoid_op_plus)}.
-
-  (** ** Boring admitted lemmas *)
-  (******************************************************************************)
-  Lemma lc_bound: forall t e n,
-      LC (U := U) t ->
-      (e, Bd n) ∈d t ->
-      bound n e = true.
-  Proof.
-    introv HLC Hin. cbn.
-    unfold LC, LCn in HLC.
-    specialize (HLC e (Bd n) Hin).
-    unfold lc_loc in HLC.
-    replace (e + 0) with e in * by lia.
-    destruct e.
-    lia.
-    rewrite PeanoNat.Nat.leb_le. lia.
-  Qed.
-
-  Lemma bound_in_plus: forall n depth,
-      bound (n + depth) depth = false.
-  Proof.
-    intros. destruct depth.
-    - reflexivity.
-    - cbn.
-      rewrite Compare_dec.leb_iff_conv.
-      lia.
-  Qed.
-
-  Lemma toDB_Fr: forall (n: nat) (a: atom) (k: key),
-      a ∈ k ->
-      exists ix, toDB_loc k (n, Fr a) = Some ix.
-  Proof.
-    intros.
-    unfold toDB_loc.
-    lookup atom a in key k.
-    rewrite H_key_lookup.
-    eexists. reflexivity.
-  Qed.
-
-  (** ** Supporting lemmas *)
-  (******************************************************************************)
-  Definition whole_key (t: U LN) (k: key) :=
-    forall x : atom, Fr x ∈ t -> x ∈ k.
-
-  (** ** LN to DB to LN *)
-  (******************************************************************************)
-  Lemma to_DB_from_key_total:
-    forall (t: U LN) (k : key),
-      whole_key t k ->
-      exists (t': U nat), toDB_from_key k t = Some t'.
-  Proof.
-    introv Hin.
-    unfold toDB_from_key.
-    rewrite DecoratedTraversableFunctor.mapdt_through_runBatch.
-    unfold compose at 1.
-    unfold whole_key in Hin.
-    unfold element_of in Hin.
-    rewrite (tosubset_through_runBatch2 _ nat) in Hin.
-    rewrite toBatch_to_toBatch3 in Hin.
-    unfold compose in Hin.
-    induction (toBatch3 t).
-    - cbv. eauto.
-    - rewrite runBatch_rw2.
-      assert (H: (forall x : atom,
-                     @runBatch LN nat (@const Type Type (LN -> Prop))
-                       (@Map_const (LN -> Prop))
-                       (@Mult_const (LN -> Prop) (@Monoid_op_subset LN))
-                       (@Pure_const (LN -> Prop) (@Monoid_unit_subset LN))
-                       (@ret subset Return_subset LN) (nat -> C)
-                       (@mapfst_Batch nat (nat -> C) (nat * LN) LN
-                          (@extract (prod nat) (Extract_reader nat) LN) b)
-                       (Fr x) -> x ∈ k)).
-      { intros x.
-        specialize (Hin x).
-        intros hyp.
-        apply Hin.
-        left.
-        assumption. }
-      specialize (IHb H).
-      destruct IHb as [f Hfeq].
-      rewrite Hfeq.
-      destruct a as [depth l].
-      destruct l.
-      + pose toDB_Fr.
-        specialize (e depth n k).
-        enough (H_a_in_k: n ∈ k).
-        { specialize (e H_a_in_k).
-          destruct e as [ix Hixeq].
-          rewrite Hixeq.
-          cbn.
-          eauto. }
-        apply Hin.
-        cbn. right.
-        reflexivity.
-      + cbn. eauto.
-  Qed.
-
-  Lemma LN_DB_roundtrip_loc1: forall k depth x,
-      x ∈ k ->
-      map (F := option)
-        (toLN_loc k ∘ pair depth ∘ (fun ix : nat => ix + depth))
-        (key_lookup_atom k x) = Some (Some (Fr x)).
-  Proof.
-    intros.
-    lookup atom x in key k.
-    rewrite H_key_lookup.
-    change (map ?f (Some ?n)) with (Some (f n)).
-    unfold compose, toLN_loc.
-    rewrite bound_in_plus.
-    replace (n + depth - depth) with n by lia.
-    rewrite (key_bijection1 x k n H_key_lookup).
-    reflexivity.
-  Qed.
-
-  Lemma LN_DB_roundtrip_loc: forall t k depth l,
-      LC t ->
-      whole_key t k ->
-      (depth, l) ∈d t ->
-      (toLN_loc k ⋆3 toDB_loc k) (depth, l) = pure (F := option ∘ option) l.
-  Proof.
-    introv Hlc Hwhole Hin.
-    rewrite kc3_spec.
-    unfold whole_key in Hwhole.
-    destruct l as [x|n].
-    - rewrite toDB_loc_rw2.
-      compose near (key_lookup_atom k x).
-      rewrite (fun_map_map (F := option)).
-      apply ind_implies_in in Hin.
-      specialize (Hwhole x Hin); clear Hin.
-      now apply LN_DB_roundtrip_loc1.
-    - rewrite toDB_loc_rw1.
-      change (map ?f (Some ?n)) with (Some (f n)).
-      unfold compose.
-      unfold toLN_loc.
-      now rewrite (lc_bound t depth n Hlc Hin).
-  Qed.
-
-  Theorem LN_DB_roundtrip:
-    forall (t : U LN) (k: key),
-      (forall x : atom, Fr x ∈ t -> x ∈ k) ->
-      LC t ->
-      map (F := option) (toLN_from_key k) (toDB_from_key k t) =
-        Some (Some t).
-  Proof.
-    intros.
-    unfold toLN_from_key.
-    unfold toDB_from_key.
-    compose near t on left.
-    rewrite mapdt_mapdt.
-    all: try typeclasses eauto.
-    change (Some (Some t)) with (pure (F := option ∘ option) t).
-    apply (mapdt_respectful_pure _ (G := option ∘ option)).
-    intros.
-    now rewrite (LN_DB_roundtrip_loc t).
-  Qed.
-
-  (** ** DB to LN to DB *)
-  (******************************************************************************)
-  Lemma DB_LN_roundtrip_loc1:
-    forall (t:U nat) k gap depth (n:nat),
-      unique k ->
-      cl_at gap t ->
-      contains_ix_upto gap k ->
-      bound n depth = false ->
-      (depth, n) ∈d t ->
-      map (toDB_loc k ∘ pair depth) (map Fr (key_lookup_index k (n - depth))) = Some (Some n).
-  Proof.
-    introv Huniq Hclosed Hcont Hbound Helt.
-    unfold toLN_loc.
-    assert (Hcont_minus: contains_ix_upto (n - depth) k).
-    { clear Hbound.
-      unfold contains_ix_upto in *.
-      (* assert (n - depth <= gap).*)
-      unfold cl_at in Hclosed;
-        specialize (Hclosed depth n Helt);
-        clear Helt;
-        unfold cl_at_loc in Hclosed;
-        unfold bound_within in Hclosed;
-        rewrite PeanoNat.Nat.ltb_lt in Hclosed.
-      lia.
-    }
-    {
-      unfold bound, bound_within in Hbound;
-        rewrite PeanoNat.Nat.ltb_ge in Hbound;
-        replace (depth + 0) with depth in Hbound by lia.
-      destruct (key_lookup_ix_Some2 k (n-depth) Hcont_minus) as [a Halookup].
-      rewrite Halookup.
-      change (map ?f (Some ?n)) with (Some (f n)).
-      change (map ?f (Some ?n)) with (Some (f n)).
-      cbn.
-      apply (key_bijection2) in Halookup; auto.
-      rewrite Halookup; clear Halookup.
-      change (map ?f (Some ?n)) with (Some (f n)).
-      cbn.
-      replace (n - depth + depth) with n by lia.
-      reflexivity.
-    }
-  Qed.
-
-  Lemma DB_LN_roundtrip_loc: forall (t:U nat) k gap depth (n:nat),
-      unique k ->
-      cl_at gap t ->
-      contains_ix_upto gap k ->
-      (depth, n) ∈d t ->
-      (toDB_loc k ⋆3 toLN_loc k) (depth, n) =
-        pure (F := option ∘ option) n.
-  Proof.
-    introv Huniq Hclosed Hcont Helt.
-    unfold_ops @Pure_compose @Pure_option.
-    rewrite kc3_spec.
-    unfold toLN_loc.
-    bound_induction.
-    apply (DB_LN_roundtrip_loc1 t k gap depth n
-             Huniq Hclosed Hcont Hbound Helt).
-  Qed.
-
-  Theorem DB_LN_roundtrip: forall k gap (t: U nat),
-      unique k ->
-      cl_at gap t ->
-      contains_ix_upto gap k ->
-      map (F := option) (toDB_from_key k) (toLN_from_key k t) =
-        Some (Some t).
-  Proof.
-    intros.
-    unfold toLN_from_key.
-    unfold toDB_from_key.
-    compose near t on left.
-    rewrite mapdt_mapdt.
-    all: try typeclasses eauto.
-    change (Some (Some t)) with (pure (F := option ∘ option) t).
-    apply (mapdt_respectful_pure _ (G := option ∘ option)).
-    intros.
-    now rewrite (DB_LN_roundtrip_loc t k gap).
-  Qed.
-
-End translate.
