Tealeaves/Backends/Adapters/DBtoLN.v
@@ -1,0 +1,47 @@
+(*|
+############################################################
+Translating between locally nameless and de Bruijn indices
+############################################################
+
+We reason about a translation between syntax with de Bruijn indices
+and locally nameless variables. This consists of a function which,
+given a locally closed term t, outputs a term of the same shape whose
+leaves are de Bruijn indices and a "key": some arbitrary permutation
+of the names of free variables in t. Another function accepts a key
+and a de Bruijn term and computes a locally nameless term of the same
+shape. The two functions are shown to be inverses.
+
+.. contents:: Table of Contents :depth: 2
+
+============================
+Imports and setup
+============================
+
+Since we are using the Kleisli typeclass hierarchy, we import modules
+under the namespaces ``Classes.Kleisli`` and ``Theory.Kleisli.``
+|*)
+From Tealeaves Require Import
+  Backends.LN
+  Backends.DB.DB
+  Backends.Adapters.Key
+  Classes.Kleisli.DecoratedTraversableFunctor
+  Functors.Option.
+
+#[local] Generalizable Variables W T U.
+#[local] Open Scope nat_scope.
+
+(*|
+============================
+Operations
+============================
+|*)
+Definition toLN_loc (k: key) '(depth, ix) : option LN :=
+  if bound ix depth == true
+  then
+    Some (Bd ix)
+  else
+    map (F := option) Fr (key_lookup_index k (ix - depth)).
+
+Definition toLN_from_key
+  `{Mapdt_inst: Mapdt nat T} (k: key): T nat -> option (T LN) :=
+  mapdt (G := option) (toLN_loc k).
