Tealeaves/Backends/Adapters/Roundtrips/LNDB.v
@@ -1,0 +1,402 @@
+(*|
+############################################################
+Translating between locally nameless and de Bruijn indices
+############################################################
+
+We reason about a translation between syntax with de Bruijn indices
+and locally nameless variables. This consists of a function which,
+given a locally closed term t, outputs a term of the same shape whose
+leaves are de Bruijn indices and a "key": some arbitrary permutation
+of the names of free variables in t. Another function accepts a key
+and a de Bruijn term and computes a locally nameless term of the same
+shape. The two functions are shown to be inverses.
+
+.. contents:: Table of Contents :depth: 2
+
+============================
+Imports and setup
+============================
+
+Since we are using the Kleisli typeclass hierarchy, we import modules
+under the namespaces ``Classes.Kleisli`` and ``Theory.Kleisli.``
+|*)
+From Tealeaves Require Import
+  Backends.LN
+  Backends.DB.DB
+  Backends.Adapters.Key
+  Backends.Adapters.LNtoDB
+  Backends.Adapters.DBtoLN
+  Functors.Option.
+
+Import LN.Notations.
+
+Import DecoratedTraversableMonad.UsefulInstances.
+
+#[local] Generalizable Variables W T U.
+#[local] Open Scope nat_scope.
+
+
+Section translate.
+
+  Context
+    `{Return_T: Return T}
+    `{Binddt_TT: Binddt nat T T}
+    `{Binddt_TU: Binddt nat T U}
+    `{Monad_inst: ! DecoratedTraversableMonad nat T}
+    `{Module_inst: ! DecoratedTraversableRightPreModule nat T U
+    (unit := Monoid_unit_zero)
+    (op := Monoid_op_plus)}.
+
+  (** ** Basic supporting lemmas *)
+  (********************************************************************)
+  Lemma lc_bound: forall t e n,
+      LC (U := U) t ->
+      (e, Bd n) ∈d t ->
+      bound n e = true.
+  Proof.
+    introv HLC Hin. cbn.
+    unfold LC, LCn in HLC.
+    specialize (HLC e (Bd n) Hin).
+    unfold lc_loc in HLC.
+    replace (e + 0) with e in * by lia.
+    destruct e.
+    lia.
+    rewrite PeanoNat.Nat.leb_le. lia.
+  Qed.
+
+  Lemma bound_in_plus: forall n depth,
+      bound (n + depth) depth = false.
+  Proof.
+    intros. destruct depth.
+    - reflexivity.
+    - cbn.
+      rewrite Compare_dec.leb_iff_conv.
+      lia.
+  Qed.
+
+  Lemma toDB_Fr: forall (n: nat) (a: atom) (k: key),
+      a ∈ k ->
+      exists ix, toDB_loc k (n, Fr a) = Some ix.
+  Proof.
+    intros.
+    unfold toDB_loc.
+    lookup atom a in key k.
+    rewrite H_key_lookup.
+    eexists. reflexivity.
+  Qed.
+
+  Definition scoped_key (t: U LN) (k: key) :=
+    forall x: atom, Fr x ∈ t -> x ∈ k.
+
+  (** ** Totality *)
+  (********************************************************************)
+  (** Given a locally nameless term and a key with enough atoms,
+      <<toDB>> is guaranteed to return something. *)
+  Lemma to_DB_from_key_total:
+    forall (t: U LN) (k: key),
+      scoped_key t k ->
+      exists (t': U nat), toDB_from_key k t = Some t'.
+  Proof.
+    introv Hin.
+    unfold toDB_from_key.
+    rewrite DecoratedTraversableFunctor.mapdt_through_runBatch.
+    unfold compose at 1.
+    unfold scoped_key in Hin.
+    unfold element_of in Hin.
+    rewrite (tosubset_through_runBatch2 _ nat) in Hin.
+    rewrite toBatch_to_toBatch3 in Hin.
+    unfold compose in Hin.
+    induction (toBatch3 t).
+    - cbv. eauto.
+    - rewrite runBatch_rw2.
+      assert (H: (forall x: atom,
+                     @runBatch LN nat (@const Type Type (LN -> Prop))
+                       (@Map_const (LN -> Prop))
+                       (@Mult_const (LN -> Prop) (@Monoid_op_subset LN))
+                       (@Pure_const (LN -> Prop) (@Monoid_unit_subset LN))
+                       (@ret subset Return_subset LN) (nat -> C)
+                       (@mapfst_Batch nat (nat -> C) (nat * LN) LN
+                          (@extract (prod nat) (Extract_reader nat) LN) b)
+                       (Fr x) -> x ∈ k)).
+      { intros x.
+        specialize (Hin x).
+        intros hyp.
+        apply Hin.
+        left.
+        assumption. }
+      specialize (IHb H).
+      destruct IHb as [f Hfeq].
+      rewrite Hfeq.
+      destruct a as [depth l].
+      destruct l.
+      + pose toDB_Fr.
+        specialize (e depth n k).
+        enough (H_a_in_k: n ∈ k).
+        { specialize (e H_a_in_k).
+          destruct e as [ix Hixeq].
+          rewrite Hixeq.
+          cbn.
+          eauto. }
+        apply Hin.
+        cbn. right.
+        reflexivity.
+      + cbn. eauto.
+  Qed.
+
+  Lemma mapdt_None:
+    forall (A B: Type) (t: T A) (f: nat * A -> option B),
+      (exists (n: nat) (a: A), (n, a) ∈d t /\ f (n, a) = None) ->
+      mapdt f t = None.
+  Proof.
+    intros.
+    rewrite mapdt_through_runBatch.
+  Abort.
+
+  Lemma to_DB_from_key_None:
+    forall (t: U LN) (k: key),
+      (exists (x: atom), Fr x ∈ t /\ ~ x ∈ k) ->
+      toDB_from_key k t = None.
+  Proof.
+    intros. unfold scoped_key in H.
+  Abort.
+
+
+  (** ** Roundtrip from LN *)
+  (********************************************************************)
+
+  (** A helper lemma used below *)
+  Lemma LN_DB_roundtrip_loc_helper1: forall k depth x,
+      x ∈ k ->
+      map (F := option)
+        (toLN_loc k ∘ pair depth ∘ (fun ix: nat => ix + depth))
+        (key_lookup_atom k x) = Some (Some (Fr x)).
+  Proof.
+    intros.
+    lookup atom x in key k.
+    rewrite H_key_lookup.
+    change (map ?f (Some ?n)) with (Some (f n)).
+    unfold compose, toLN_loc.
+    rewrite bound_in_plus.
+    replace (n + depth - depth) with n by lia.
+    rewrite (key_bijection1 x k n H_key_lookup).
+    reflexivity.
+  Qed.
+
+  (** Starting with a locally closed term and a big enough key,
+      the roundtrip is locally the identity function *)
+  Lemma LN_DB_roundtrip_loc: forall t k depth l,
+      LC t ->
+      scoped_key t k ->
+      (depth, l) ∈d t ->
+      (toLN_loc k ⋆3 toDB_loc k) (depth, l) = pure (F := option ∘ option) l.
+  Proof.
+    introv Hlc Hwhole Hin.
+    rewrite kc3_spec.
+    unfold scoped_key in Hwhole.
+    destruct l as [x|n].
+    - rewrite toDB_loc_rw2.
+      compose near (key_lookup_atom k x).
+      rewrite (fun_map_map (F := option)).
+      apply ind_implies_in in Hin.
+      specialize (Hwhole x Hin); clear Hin.
+      now apply LN_DB_roundtrip_loc_helper1.
+    - rewrite toDB_loc_rw1.
+      change (map ?f (Some ?n)) with (Some (f n)).
+      unfold compose.
+      unfold toLN_loc.
+      now rewrite (lc_bound t depth n Hlc Hin).
+  Qed.
+
+  (** Starting with a locally closed term and a big enough key,
+      the roundtrip is locally the identity function *)
+  Theorem LN_DB_roundtrip:
+    forall (t: U LN) (k: key),
+      (forall x: atom, Fr x ∈ t -> x ∈ k) ->
+      LC t ->
+      map (F := option) (toLN_from_key k) (toDB_from_key k t) =
+        Some (Some t).
+  Proof.
+    intros.
+    unfold toLN_from_key.
+    unfold toDB_from_key.
+    compose near t on left.
+    rewrite mapdt_mapdt.
+    all: try typeclasses eauto.
+    change (Some (Some t)) with (pure (F := option ∘ option) t).
+    apply (mapdt_respectful_pure _ (G := option ∘ option)).
+    intros.
+    now rewrite (LN_DB_roundtrip_loc t).
+  Qed.
+
+  (** ** Roundtrip from DB *)
+  (********************************************************************)
+
+  (** A helper lemma used below *)
+  Lemma DB_LN_roundtrip_loc_helper1:
+    forall (t:U nat) k gap depth (n:nat),
+      unique k ->
+      cl_at gap t ->
+      contains_ix_upto gap k ->
+      bound n depth = false ->
+      (depth, n) ∈d t ->
+      map (toDB_loc k ∘ pair depth) (map Fr (key_lookup_index k (n - depth))) = Some (Some n).
+  Proof.
+    introv Huniq Hclosed Hcont Hbound Helt.
+    unfold toLN_loc.
+    assert (Hcont_minus: contains_ix_upto (n - depth) k).
+    { clear Hbound.
+      unfold contains_ix_upto in *.
+      (* assert (n - depth <= gap).*)
+      unfold cl_at in Hclosed;
+        specialize (Hclosed depth n Helt);
+        clear Helt;
+        unfold cl_at_loc in Hclosed;
+        unfold bound_within in Hclosed;
+        rewrite PeanoNat.Nat.ltb_lt in Hclosed.
+      lia.
+    }
+    {
+      unfold bound, bound_within in Hbound;
+        rewrite PeanoNat.Nat.ltb_ge in Hbound;
+        replace (depth + 0) with depth in Hbound by lia.
+      destruct (key_lookup_ix_Some2 k (n-depth) Hcont_minus) as [a Halookup].
+      rewrite Halookup.
+      change (map ?f (Some ?n)) with (Some (f n)).
+      change (map ?f (Some ?n)) with (Some (f n)).
+      cbn.
+      apply (key_bijection2) in Halookup; auto.
+      rewrite Halookup; clear Halookup.
+      change (map ?f (Some ?n)) with (Some (f n)).
+      cbn.
+      replace (n - depth + depth) with n by lia.
+      reflexivity.
+    }
+  Qed.
+
+  (** A helper lemma used below *)
+  Lemma DB_LN_roundtrip_loc: forall (t:U nat) k gap depth (n:nat),
+      unique k ->
+      cl_at gap t ->
+      contains_ix_upto gap k ->
+      (depth, n) ∈d t ->
+      (toDB_loc k ⋆3 toLN_loc k) (depth, n) =
+        pure (F := option ∘ option) n.
+  Proof.
+    introv Huniq Hclosed Hcont Helt.
+    unfold_ops @Pure_compose @Pure_option.
+    rewrite kc3_spec.
+    unfold toLN_loc.
+    bound_induction.
+    apply (DB_LN_roundtrip_loc_helper1 t k gap depth n
+             Huniq Hclosed Hcont Hbound Helt).
+  Qed.
+
+  (** Starting with a term with no more than <<gap>>-level free variables, if the key has at least <<gap>> many unique
+      names, the roundtrip of a de Bruijn index is locally the identity function. *)
+  Theorem DB_LN_roundtrip: forall k gap (t: U nat),
+      unique k ->
+      cl_at gap t ->
+      contains_ix_upto gap k ->
+      map (F := option) (toDB_from_key k) (toLN_from_key k t) =
+        Some (Some t).
+  Proof.
+    intros.
+    unfold toLN_from_key.
+    unfold toDB_from_key.
+    compose near t on left.
+    rewrite mapdt_mapdt.
+    all: try typeclasses eauto.
+    change (Some (Some t)) with (pure (F := option ∘ option) t).
+    apply (mapdt_respectful_pure _ (G := option ∘ option)).
+    intros.
+    now rewrite (DB_LN_roundtrip_loc t k gap).
+  Qed.
+
+  (** ** Partial Bijections *)
+  (********************************************************************)
+  Theorem partial_bijection_spec1:
+    forall (A B: Type) (f: A -> option B) (g: B -> option A),
+      (forall (a: A), f a = None \/ map g (f a) = Some (Some a)) ->
+      (forall (b: B), g b = None \/ map f (g b) = Some (Some b)) ->
+      (forall (a: A) (b: B), f a = Some b <-> g b = Some a).
+  Proof.
+    introv HA HB.
+    intros a b.
+    split.
+    - intros Hf.
+      specialize (HA a).
+      rewrite Hf in HA.
+      cbn in HA.
+      inversion HA.
+      + inversion H.
+      + inversion H.
+        reflexivity.
+    - intros Hg.
+      specialize (HB b).
+      rewrite Hg in HB.
+      cbn in HB.
+      inversion HB.
+      + inversion H.
+      + inversion H.
+        reflexivity.
+  Qed.
+
+  Theorem partial_bijection_spec2:
+    forall (A B: Type) (f: A -> option B) (g: B -> option A),
+      (forall (a: A) (b: B), f a = Some b <-> g b = Some a) ->
+      (forall (a: A), f a = None \/ map g (f a) = Some (Some a)).
+  Proof.
+    introv H. intro a.
+    specialize (H a).
+    destruct (f a) as [b|].
+    - right.
+      destruct (H b) as [H1 _].
+      specialize (H1 ltac:(reflexivity)).
+      cbn. fequal.
+      assumption.
+    - now left.
+  Qed.
+
+  Theorem partial_bijection_spec3:
+    forall (A B: Type) (f: A -> option B) (g: B -> option A),
+      (forall (a: A) (b: B), f a = Some b <-> g b = Some a) ->
+      (forall (b: B), g b = None \/ map f (g b) = Some (Some b)).
+  Proof.
+    introv H. intro b.
+    remember (g b) as gb.
+    destruct gb as [a|].
+    - right.
+      cbn.
+      fequal.
+      apply H.
+      symmetry.
+      assumption.
+    - now left.
+  Qed.
+
+  Theorem partial_bijection_spec:
+    forall (A B: Type) (f: A -> option B) (g: B -> option A),
+      (forall (a: A) (b: B), f a = Some b <-> g b = Some a) <->
+      (forall (b: B), g b = None \/ map f (g b) = Some (Some b)) /\
+        (forall (a: A), f a = None \/ map g (f a) = Some (Some a)).
+  Proof.
+    intros. split.
+    - intros. split.
+      now apply partial_bijection_spec2.
+      now apply partial_bijection_spec3.
+    - intros [H1 H2].
+      apply partial_bijection_spec1.
+      assumption.
+      assumption.
+  Qed.
+
+  Theorem DB_LN_partial_bijection1: forall k,
+      (forall (t: T LN) (u: T nat),
+          toDB_from_key k t = Some u <-> toLN_from_key k u = Some t).
+  Proof.
+    intros.
+    cbn.
+  Abort.
+
+End translate.
+
